chore: cleanup term types

lib/Literal.lean
@@ -1,21 +1,37 @@
 import lib.NamedNode
 import lib.vocab
-import LeanCopilot
 
 structure LanguageTaggedStringLiteral where
   value : String
   language : String
-deriving Repr, BEq
+deriving DecidableEq
+
+instance : ToString LanguageTaggedStringLiteral where
+  toString s := "\"" ++ s.value ++ "\"@" ++ s.language
+
+instance : Repr LanguageTaggedStringLiteral where
+  reprPrec s _ := toString s
 
 structure TypedLiteral where
   value : String
   datatype : NamedNode
-deriving Repr, BEq
+deriving DecidableEq
+
+instance : ToString TypedLiteral where
+  toString s := "\"" ++ s.value ++ "\"^^" ++ (toString s.datatype)
+
+instance : Repr TypedLiteral where
+  reprPrec s _ := toString s
 
 inductive Literal where
   | LanguageTaggedString : LanguageTaggedStringLiteral → Literal
   | Typed : TypedLiteral → Literal
-deriving Repr, BEq
+deriving Repr, DecidableEq
+
+instance : ToString Literal where
+  toString : Literal → String
+    | Literal.LanguageTaggedString l => toString l
+    | Literal.Typed l => toString l
 
 def Literal.toTyped? : Literal → (Option TypedLiteral)
   | Literal.Typed l => some l
@@ -32,7 +48,7 @@ instance : Coe LanguageTaggedStringLiteral Literal where coe := Literal.Language
 -- FIXME: This is to help along nested optionals
 -- see https://leanprover.zulipchat.com/#narrow/stream/113488-general/topic/.E2.9C.94.20Coercing.20recursive.20.60Option.60s/near/422643899
 instance [Coe TypedLiteral (Option α)] : Coe Literal (Option α) where
-  coe a := match (a: Option TypedLiteral) with
+  coe a := match Literal.toTyped? a with
     | some l => l
     | _ => none
 
@@ -43,84 +59,23 @@ def TypedLiteral.toInt? (literal: TypedLiteral): Option Int :=
   if literal.datatype == XSD.integer then String.toInt? literal.value else none
 instance : Coe TypedLiteral (Option Int) where coe := TypedLiteral.toInt?
 
-theorem stringToIntRoundtrip (x: Int) : (String.toInt? (toString x)) = some x := by sorry
-
--- theorem stringToIntRoundtrip (x: Int) (i: String.Pos) (h1: y = toString x) (h2: i. ≤ y.length) (h3: i ≥ 0) : (String.toInt? (y.)) = some x := by
---   simp [String.toInt?]
---   induction x
---   case zero => exact rfl
---   case succ x ih => exact ih
-
--- theorem isNatRoundTrip (x: Nat) : (String.isNat (toString x)) = true := by
---   cases x
---   case zero => exact rfl
---   case succ x ih => simp [toString, Nat.repr, String.isNat]
-  -- simp [ toString, Nat.repr ]
-
-  -- simp [toString, Nat.repr, Nat.toDigits, Nat.toDigitsCore, Nat.digitChar, Char.ofNat, String.utf8ByteSize, Nat.isValidChar, String.isNat, Char.isDigit, String.all, String.isEmpty, String.endPos, List.asString, Nat.toDigits, Nat.toDigitsCore, Nat.digitChar, Char.ofNat, String.utf8ByteSize, Nat.isValidChar, String.utf8ByteSize.go, Char.ofNatAux, UInt32.size]
-  -- simp
-  -- exact rfl
-
-
-  -- search_proof
-  -- simp [String.isNat, Char.isDigit, String.all, String.isEmpty, String.endPos, List.asString, Nat.toDigits, Nat.toDigitsCore, Nat.digitChar, Char.ofNat, String.utf8ByteSize, Nat.isValidChar];
-  -- decide
-  -- exact ⟨by decide, by decide ⟩
-  -- cases toString x <;>
-  -- simp [toString ]
-  -- simp [toString, String.all ]
-  -- simp [String.isEmpty ]
-  -- simp [String.all ]
-  -- unfold  String.isEmpty
-  -- simp [toString, toString ]
-  -- simp [String.all, toString ]
-  -- unfold  String.all
-  -- unfold  toString
-  -- cases x <;>  decide
-  -- cases toString  x
-  -- cases toString x <;>  simp!
-  -- constructor <;>  intro
-  --  trivial
-  -- constructor <;> intro  h
-  -- constructor <;>  simp
-  --  constructor
-  -- cases  x
-  -- suggest_tactics
-  -- suggest_tactics
-  -- induction x
-  -- case zero => exact rfl
-  -- case succ x ih => simp [toString, Nat.repr]
-
-  -- simp [String.isNat, Char.isDigit];
-  -- -- simp [String.isNat, toString, Nat.repr, String.isEmpty, String.endPos, List.asString, Nat.toDigits, Nat.toDigitsCore, Nat.digitChar, Char.ofNat, String.utf8ByteSize, Nat.isValidChar, ]
-
-  -- -- simp [String.isNat, toString, Nat.repr, String.isEmpty, String.endPos, List.asString, Nat.toDigits, Nat.toDigitsCore, Nat.digitChar, Char.ofNat, String.utf8ByteSize, Nat.isValidChar, ]
-
-  -- induction x
-  -- case zero => exact rfl
-  -- case succ x ih => exact ih
-
--- theorem stringToNatRoundtrip (x: Nat) : (String.toNat? (toString x)) = some x := by
---   simp [String.toNat?]
---   induction x
---   case zero => exact rfl
---   case succ x ih =>
-
-  -- cases (String.toNat? (toString x)) with
-  --   | none => exact rfl
-  --   | some y => exact ih
-  -- exact (stringToNatRoundtrip x)
-
-
+theorem stringToIntRoundTrip (x: Int) : (String.toInt? (toString x)) = some x := by sorry
 theorem intInverse (x: Int) : (TypedLiteral.toInt? (Int.toTypedLiteral x)) = some x := by
   simp [TypedLiteral.toInt?, Int.toTypedLiteral]
-  exact (stringToIntRoundtrip x)
+  exact (stringToIntRoundTrip x)
+theorem intEq (x y: Int) (h1: x = y) : Int.toTypedLiteral x = Int.toTypedLiteral y := by simp [Int.toTypedLiteral, h1]
+theorem intEqInv (x y: Int) (h1: Int.toTypedLiteral x = Int.toTypedLiteral y) : x = y := by
+  simp [Int.toTypedLiteral] at h1
+  have h2: (String.toInt? (toString x)) = some x := stringToIntRoundTrip x
+  rw [h1, stringToIntRoundTrip y] at h2;
+  simp [some] at h2;
+  exact h2.symm;
 
 def Bool.toTypedLiteral (i: Bool): TypedLiteral := ⟨toString i, XSD.boolean⟩
 instance : Coe Bool TypedLiteral where coe := Bool.toTypedLiteral
 
 def TypedLiteral.toBool? (literal: TypedLiteral): Option Bool :=
-  if literal.datatype == XSD.boolean then
+  if literal.datatype = XSD.boolean then
     match literal.value.toLower with
     | "true" | "1" => some true
     | "false" | "0" => some false
@@ -129,18 +84,32 @@ def TypedLiteral.toBool? (literal: TypedLiteral): Option Bool :=
 instance : Coe TypedLiteral (Option Bool) where coe := TypedLiteral.toBool?
 
 theorem boolInverse (x: Bool) : (TypedLiteral.toBool? (Bool.toTypedLiteral x)) = some x := by cases x <;> exact rfl
+-- TODO: Use notions of injectivity here
+theorem boolEq (x y: Bool) (h1: x = y) : Bool.toTypedLiteral x = Bool.toTypedLiteral y := by simp [Bool.toTypedLiteral, h1]
+theorem boolEqInv (x y: Bool) (h1: Bool.toTypedLiteral x = Bool.toTypedLiteral y) : x = y := by
+  simp [Bool.toTypedLiteral] at h1
+  cases x; cases y;
+  simp [toString] at h1;
+  simp;
+  simp [toString] at h1;
+  contradiction
+  cases y;
+  simp [toString] at h1;
+  contradiction;
+  simp [toString] at h1;
+  simp;
 
 instance : Coe Float TypedLiteral where coe s := ⟨toString s, XSD.float⟩
--- FIXME: Implement reverse direction
 
 def String.toTypedLiteral (s: String): TypedLiteral := ⟨s, XSD.string⟩
 instance : Coe String TypedLiteral where coe := String.toTypedLiteral
 
-def TypedLiteral.toString? (literal: TypedLiteral): Option String :=
-  if literal.datatype == XSD.string then some literal.value else none
+def TypedLiteral.toString? (literal: TypedLiteral): Option String := if literal.datatype = XSD.string then some literal.value else none
 instance : Coe TypedLiteral (Option String) where coe := TypedLiteral.toString?
 
 theorem stringInverse (x: String) : (TypedLiteral.toString? (String.toTypedLiteral x)) = some x := by exact rfl
+theorem stringEq (x y: String) (h1: x = y) : String.toTypedLiteral x = String.toTypedLiteral y := by simp [String.toTypedLiteral, h1]
+theorem stringEqInv (x y: String) (h1: String.toTypedLiteral x = String.toTypedLiteral y) : x = y := by simp [String.toTypedLiteral] at h1; exact h1
 
 instance : Coe UInt8 TypedLiteral  where coe s := ⟨toString s, XSD.integer⟩
 instance : Coe UInt16 TypedLiteral where coe s := ⟨toString s, XSD.integer⟩
