lib/BlankNode.lean
@@ -1,0 +1,9 @@
+structure BlankNode where
+  id : String
+deriving Repr, DecidableEq
+
+instance : ToString BlankNode where
+  toString s := "_:" ++ s.id
+
+instance : Repr BlankNode where
+  reprPrec s _ := toString s
