lib/NamedNode.lean
@@ -1,3 +1,9 @@
 structure NamedNode where
   iri : String
-deriving Repr, DecidableEq
+deriving DecidableEq
+
+instance : ToString NamedNode where
+  toString s := "<" ++ s.iri ++ ">"
+
+instance : Repr NamedNode where
+  reprPrec s _ := toString s
