lib/Triple.lean
@@ -1,0 +1,36 @@
+import lib.BlankNode
+import lib.NamedNode
+import lib.Literal
+
+inductive Subject where
+  | NamedNode : NamedNode → Subject
+  | BlankNode : BlankNode → Subject
+deriving Repr, DecidableEq
+
+instance : ToString Subject where
+  toString : Subject → String
+  | Subject.NamedNode s => toString s
+  | Subject.BlankNode s => toString s
+
+inductive Object where
+  | NamedNode : NamedNode → Object
+  | BlankNode : BlankNode → Object
+  | Literal : Literal → Object
+deriving Repr, DecidableEq
+
+instance : ToString Object where
+  toString : Object → String
+  | Object.NamedNode s => toString s
+  | Object.BlankNode s => toString s
+  | Object.Literal s => toString s
+
+structure Triple where
+  subject : Subject
+  predicate : NamedNode
+  object : Object
+deriving Repr, DecidableEq
+
+instance : ToString Triple where
+  toString triple := "(" ++ toString triple.subject ++ ", " ++ toString triple.predicate ++ ", " ++ toString triple.object ++ ")"
+
+#eval toString (⟨Subject.NamedNode ⟨"http://example.com/subject"⟩, ⟨"http://example.com/predicate"⟩, Object.Literal ((1:):)⟩ : Triple)
